lakefile.lean
@@ -10,7 +10,7 @@ require mathlib from git
   "https://github.com/leanprover-community/mathlib4.git" @ "v4.32.1"
 
 require jaune from git
-  "https://github.com/skbaek/jaune.git" @ "4b2171d8f7b5324482332d38d3d9efee01764743"
+  "https://github.com/skbaek/jaune.git" @ "739fa42d23c91d3add313437dde5648cf182428b"
 
 @[default_target]
 lean_lib «Blanc» where
