scripts/AxiomCheck.lean
@@ -4,3 +4,4 @@ import Blanc.Solvent
 #print axioms Blanc.stateTransition_preserves_solvent
 #print axioms Blanc.chain_preserves_solvent
 #print axioms Blanc.addBlockToChain_preserves_solvent
+#print axioms Blanc.stateTransitionUsing_preserves_solvent
